silveroak-opentitan/hmac/Spec/Tests/HMACTests.v
@@ -16,9 +16,10 @@
 
 Require Import Coq.Lists.List.
 Require Import Coq.NArith.NArith.
+Require Import Cava.Util.BitArithmetic.
 Require Import HmacSpec.HMAC.
 Require Import HmacSpec.Tests.HMACTestVectors.
-Import ListNotations.
+Import ListNotations BigEndianBytes.
 Local Open Scope N_scope.
 
 (* Uncomment the below for step-by-step tests of intermediate values for test1
@@ -26,27 +27,30 @@ Local Open Scope N_scope.
 (*
 (* Check key padding *)
 Goal (let t := test1 in
-      padded_key t.(lK) t.(K) = t.(expected_padded_key)).
+      concat_bytes (padded_key t.(K_bytes)) = t.(expected_padded_key)).
 Proof. vm_compute. reflexivity. Qed.
 
 (* Check K ^ ipad *)
 Goal (let t := test1 in
-      N.lxor t.(expected_padded_key) ipad = t.(expected_xor_K_ipad)).
+      concat_bytes (XOR (N_to_bytes B t.(expected_padded_key)) ipad)
+      = t.(expected_xor_K_ipad)).
 Proof. vm_compute. reflexivity. Qed.
 
 (* Check K ^ opad *)
 Goal (let t := test1 in
-      N.lxor t.(expected_padded_key) opad = t.(expected_xor_K_opad)).
+      concat_bytes (XOR (N_to_bytes B t.(expected_padded_key)) opad)
+      = t.(expected_xor_K_opad)).
 Proof. vm_compute. reflexivity. Qed.
 
 (* Check inner hash result *)
 Goal (let t := test1 in
-      H B t.(ldata) t.(expected_xor_K_ipad) t.(data) = t.(expected_inner)).
+      concat_bytes (H (N_to_bytes B t.(expected_xor_K_ipad)) (N_to_bytes t.(ldata) t.(data)))
+      = t.(expected_inner)).
 Proof. vm_compute. reflexivity. Qed.
 *)
 
 Goal (let t := test1 in
-      hmac_sha256 t.(lK) t.(ldata) t.(K) t.(data) = t.(expected_output)).
+      concat_bytes (hmac_sha256 t.(K_bytes) t.(data_bytes)) = t.(expected_output)).
 Proof. vm_compute. reflexivity. Qed.
 
 (* Uncomment the below for step-by-step tests of intermediate values for test2
@@ -54,27 +58,30 @@ Proof. vm_compute. reflexivity. Qed.
 (*
 (* Check key padding *)
 Goal (let t := test2 in
-      padded_key t.(lK) t.(K) = t.(expected_padded_key)).
+      concat_bytes (padded_key t.(K_bytes)) = t.(expected_padded_key)).
 Proof. vm_compute. reflexivity. Qed.
 
 (* Check K ^ ipad *)
 Goal (let t := test2 in
-      N.lxor t.(expected_padded_key) ipad = t.(expected_xor_K_ipad)).
+      concat_bytes (XOR (N_to_bytes B t.(expected_padded_key)) ipad)
+      = t.(expected_xor_K_ipad)).
 Proof. vm_compute. reflexivity. Qed.
 
 (* Check K ^ opad *)
 Goal (let t := test2 in
-      N.lxor t.(expected_padded_key) opad = t.(expected_xor_K_opad)).
+      concat_bytes (XOR (N_to_bytes B t.(expected_padded_key)) opad)
+      = t.(expected_xor_K_opad)).
 Proof. vm_compute. reflexivity. Qed.
 
 (* Check inner hash result *)
 Goal (let t := test2 in
-      H B t.(ldata) t.(expected_xor_K_ipad) t.(data) = t.(expected_inner)).
+      concat_bytes (H (N_to_bytes B t.(expected_xor_K_ipad)) (N_to_bytes t.(ldata) t.(data)))
+      = t.(expected_inner)).
 Proof. vm_compute. reflexivity. Qed.
 *)
 
 Goal (let t := test2 in
-      hmac_sha256 t.(lK) t.(ldata) t.(K) t.(data) = t.(expected_output)).
+      concat_bytes (hmac_sha256 t.(K_bytes) t.(data_bytes)) = t.(expected_output)).
 Proof. vm_compute. reflexivity. Qed.
 
 (* Uncomment the below for step-by-step tests of intermediate values for test3
@@ -82,25 +89,28 @@ Proof. vm_compute. reflexivity. Qed.
 (*
 (* Check key padding *)
 Goal (let t := test3 in
-      padded_key t.(lK) t.(K) = t.(expected_padded_key)).
+      concat_bytes (padded_key t.(K_bytes)) = t.(expected_padded_key)).
 Proof. vm_compute. reflexivity. Qed.
 
 (* Check K ^ ipad *)
 Goal (let t := test3 in
-      N.lxor t.(expected_padded_key) ipad = t.(expected_xor_K_ipad)).
+      concat_bytes (XOR (N_to_bytes B t.(expected_padded_key)) ipad)
+      = t.(expected_xor_K_ipad)).
 Proof. vm_compute. reflexivity. Qed.
 
 (* Check K ^ opad *)
 Goal (let t := test3 in
-      N.lxor t.(expected_padded_key) opad = t.(expected_xor_K_opad)).
+      concat_bytes (XOR (N_to_bytes B t.(expected_padded_key)) opad)
+      = t.(expected_xor_K_opad)).
 Proof. vm_compute. reflexivity. Qed.
 
 (* Check inner hash result *)
 Goal (let t := test3 in
-      H B t.(ldata) t.(expected_xor_K_ipad) t.(data) = t.(expected_inner)).
+      concat_bytes (H (N_to_bytes B t.(expected_xor_K_ipad)) (N_to_bytes t.(ldata) t.(data)))
+      = t.(expected_inner)).
 Proof. vm_compute. reflexivity. Qed.
  *)
 
 Goal (let t := test3 in
-      hmac_sha256 t.(lK) t.(ldata) t.(K) t.(data) = t.(expected_output)).
+      concat_bytes (hmac_sha256 t.(K_bytes) t.(data_bytes)) = t.(expected_output)).
 Proof. vm_compute. reflexivity. Qed.
